@prefix dachkg: <http://http://dachkg.org/ontology/1.0/> .
@prefix schema: <http://schema.org/> .
@prefix rdf: <http://www.w3.org/1999/02/22-rdf-syntax-ns#> .
@prefix rdfs: <http://www.w3.org/2000/01/rdf-schema#> .

##Classes


dachkg:Trail a rdfs:Class ;
    rdfs:label "Trail" ;
    rdfs:comment "A  a path, track or unpaved lane or road for sport activities or walking." ;
    rdfs:subClassOf schema:Place .


#Properties

dachkg:startLocation a rdf:Property ;
    rdfs:label "startLocation" ;
    schema:domainIncludes dachkg:Trail ;
    schema:rangeIncludes schema:Place ;
    rdfs:comment "A sub property of schema.org location. The start location of the trail." ;
    rdfs:subPropertyOf schema:location .
    
dachkg:endLocation a rdf:Property ;
    rdfs:label "endLocation" ;
    schema:domainIncludes dachkg:Trail ;
    schema:rangeIncludes schema:Place ;
    rdfs:comment "A sub property of schema.org location. The final location of the trail." ;
    rdfs:subPropertyOf schema:location .
    
dachkg:wayPoint a rdf:Property ;
    rdfs:label "wayPoints" ;
    schema:domainIncludes dachkg:Trail ;
    schema:rangeIncludes schema:Place, schema:ItemList ;
    rdfs:comment "A waypoint is an intermediate point or place or stoping point on a trail or line of travel." ;
    rdfs:subPropertyOf schema:location .
    
schema:additionalProperty a rdf:Property ;
    rdfs:label "additionalProperty" ;
    schema:domainIncludes schema:Thing,
    schema:Place,
        schema:Product,
        schema:QualitativeValue,
        schema:QuantitativeValue ;
    schema:rangeIncludes schema:PropertyValue ;
    rdfs:comment "A property-value pair representing an additional characteristics of the entitity, e.g. a product feature or another characteristic for which there is no matching property in schema.org. Note: Publishers should be aware that applications designed to use specific schema.org properties (e.g. http://schema.org/width, http://schema.org/color, http://schema.org/gtin13, ...) will typically expect such data to be provided using those properties, rather than using the generic property/value mechanism.".
   